extraction/extraction.v
@@ -108,6 +108,8 @@ Extract Constant Compopts.optim_constprop =>
   "fun _ -> !Clflags.option_fconstprop".
 Extract Constant Compopts.optim_CSE =>
   "fun _ -> !Clflags.option_fcse".
+Extract Constant Compopts.optim_CSE2 =>
+  "fun _ -> !Clflags.option_fcse2".
 Extract Constant Compopts.optim_redundancy =>
   "fun _ -> !Clflags.option_fredundancy".
 Extract Constant Compopts.thumb =>
